More progress

experiments/SmallStepExperiment.v
@@ -1,4 +1,6 @@
-From ITree Require Import ITree Trace.
+From ITree Require Import
+     ITree
+     Trace.
 
 Require Import List.
 Import ListNotations.
@@ -21,49 +23,75 @@ CoFixpoint big (s:state) : itree E state :=
 (* This doesn't work if the semantics loops because there can a nontrivial trace but these derivations can't find them *)
 Inductive big_trace : state -> (trace E) -> option state -> Prop :=
 | bt_done : forall s, done s = true -> big_trace s [] (Some s)
-| bt_tau  : forall s s' t r, ss s = inl s' -> big_trace s' t r -> big_trace s t r
+| bt_tau  : forall s s' t r, done s = false -> ss s = inl s' -> big_trace s' t r -> big_trace s t r
 | bt_vis  : forall s i e k t r,
-    ss s = inr (existT _ i (e, k)) -> forall (x:i), big_trace (k x) t r -> big_trace s ((Event e x)::t) r.
+    done s = false ->
+    ss s = inr (existT _ i (e, k)) ->
+    forall (x:i), big_trace (k x) t r -> big_trace s ((Event e x)::t) r.
 
 Fixpoint big_trace_approx (n:nat) (s:state) (t:trace E) (os:option state) : Prop :=
   match n with
-  | 0 => os = None
+  | 0 => os = None /\ t = []
   | S m =>
     (done s = true /\ os = Some s /\ t = []) \/
-    (exists s', ss s = inl s' /\ big_trace_approx m s' t os) \/
-    (exists t' i e k, ss s = inr (existT _ i (e, k))
+    (done s = false /\ exists s', ss s = inl s' /\ big_trace_approx m s' t os) \/
+    (done s = false /\ exists t' i e k, ss s = inr (existT _ i (e, k))
+                 (* exists? *)
                  /\ forall (x:i), t = ((Event e x)::t') /\ (big_trace_approx m (k x) t' os))
 end.
 
 Lemma done_big : forall s, done s = true -> big s = Ret s.
 Proof.
   intros. rewrite (itree_eta (big s)).
-  destruct (observe (big s)) eqn:?;
-           unfold big in Heqi; cbn in Heqi; rewrite H in Heqi; inversion Heqi; auto.
+  destruct (observe (big s)) eqn:Hs;
+           unfold big in Hs; cbn in Hs; rewrite H in Hs; inversion Hs; auto.
 Qed.
 
-Lemma test : forall s t os, big_trace s t os -> is_trace (big s) t os.
+Lemma not_done_big_inl : forall s s', done s = false -> ss s = inl s' -> big s = Tau (big s').
 Proof.
-  intros. induction H.
-  - rewrite (done_big _ H). constructor.
-  -
+  intros. rewrite (itree_eta (big s)).
+  destruct (observe (big s)) eqn:Hs;
+    unfold big in Hs; cbn in Hs; rewrite H in Hs; rewrite H0 in Hs; inversion Hs; auto.
+Qed.
+
+Lemma not_done_big_inr : forall s i e k,
+    done s = false ->
+    ss s = inr (existT _ i (e, k)) ->
+    big s = Vis e (fun x => big (k x)).
+Proof.
+  intros. rewrite (itree_eta (big s)).
+  destruct (observe (big s)) eqn:Hs;
+    unfold big in Hs; cbn in Hs; rewrite H in Hs; rewrite H0 in Hs; try solve [inversion Hs; subst; auto].
+  simpl in Hs. fold big in *. rewrite Hs. auto.
+Qed.
+
+Lemma test : forall s t os, big_trace s t os <-> is_trace (big s) t os.
+Proof.
+  intros. split; intros.
+  {
+    induction H.
+    - rewrite (done_big _ H). constructor.
+    - rewrite (not_done_big_inl _ _ H H0). constructor. auto.
+    - rewrite (not_done_big_inr _ _ _ _ H H0). constructor. auto.
+  }
+  {
 Admitted.
 
-(* Should this be <-> ? *)
 Lemma semantics_coincide : forall s n t os, big_trace_approx n s t os -> is_trace (big s) t os.
 Proof.
-  intros. induction n; induction t; red in H; subst.
-  - constructor.
-  - specialize (IHt eq_refl). inversion IHt; subst.
-    +
-      destruct a. eapply TraceVis.
-  - destruct H as [|[|]].
-    + decompose [and] H. subst.
-      rewrite (itree_eta (big s)). destruct (observe (big s)) eqn:?; auto.
-      * constructor 2.
+  intros s n. revert s.
+  induction n; intros.
+  - red in H. destruct H. subst. constructor.
+  - remember (S n) as n'. rewrite Heqn' in H.
+    simpl in H. decompose [or] H; clear H.
+    + decompose [and] H0; clear H0. subst. rewrite (done_big _ H). constructor.
+    + decompose [ex and] H1; clear H1. subst. rewrite (not_done_big_inl _ _ H H0).
+      constructor. auto.
+    + decompose [ex and] H1; clear H1. subst. rewrite (not_done_big_inr _ _ _ _ H H2).
+      constructor. auto.
+Qed.
 
-
-admit.
-    + decompose [ex and] H. clear H. admit.
-    + decompose [ex and] H. clear H.
+Lemma reverse: forall s t os, is_trace (big s) t os ->
+                         exists n, big_trace_approx n s t os.
+Proof.
 Admitted.
